\documentclass[12pt]{article}
\usepackage{pmmeta}
\pmcanonicalname{ExampleOfCramersRule}
\pmcreated{2013-03-22 12:50:33}
\pmmodified{2013-03-22 12:50:33}
\pmowner{drini}{3}
\pmmodifier{drini}{3}
\pmtitle{example of Cramer's rule}
\pmrecord{7}{33169}
\pmprivacy{1}
\pmauthor{drini}{3}
\pmtype{Example}
\pmcomment{trigger rebuild}
\pmclassification{msc}{15A15}

\endmetadata

\usepackage{graphicx}
%%%\usepackage{xypic} 
\usepackage{amsmath}
\usepackage{bbm}
\newcommand{\Z}{\mathbbmss{Z}}
\newcommand{\C}{\mathbbmss{C}}
\newcommand{\R}{\mathbbmss{R}}
\newcommand{\Q}{\mathbbmss{Q}}
\newcommand{\mathbb}[1]{\mathbbmss{#1}}
\newcommand{\figura}[1]{\begin{center}\includegraphics{#1}\end{center}}
\newcommand{\figuraex}[2]{\begin{center}\includegraphics[#2]{#1}\end{center}}
\begin{document}
Say we want to solve the system
\begin{eqnarray*}
3x + 2y + z -2w&=&4\\
2x - y + 2z - 5w &=& 15\\
4x + 2y \phantom{+ 2x} - 5w&=&1\\
3x \phantom{+ 2y} - 2z -4w &=& 1.
\end{eqnarray*}

The associated matrix is 
$$\begin{pmatrix}
3 & 2 & 1 & -2\\
2 & -1 & 2 & -5\\
4 & 2 & 0 & -1 \\
3 & 0 & -2 & -4
\end{pmatrix}$$

whose determinant is $\Delta=-65$. Since the determinant is non-zero, we can use Cramer's rule. To obtain the value of the $k$-th variable, we replace the $k$-th column of the matrix above by the column vector 
$$\begin{pmatrix} 4\\ 15\\ 1\\ 1\end{pmatrix},$$ 
the determinant of the obtained matrix is divided by $\Delta$ and the resulting value is the wanted solution.

So
$$
x=\frac{\Delta_1}{\Delta}=
\frac{
\begin{vmatrix}
4 & 2 & 1 & -2\\
15 & -1 & 2 & -5\\
1 & 2 & 0 & -1\\
1 & 0 & -2 & -4
\end{vmatrix}
}{-65}=\frac{-65}{-65}=1
$$

$$
y=\frac{\Delta_2}{\Delta}=
\frac{
\begin{vmatrix}
3 & 4 &  1 & -2\\
2 & 15 & 2 & -5\\
4 & 1 &  0 & -1\\
3 & 1 &  -2 & -4
\end{vmatrix}
}{-65}=\frac{130}{-65}=2
$$

$$
z=\frac{\Delta_3}{\Delta}=
\frac{
\begin{vmatrix}
3 & 2 & 4 &  -2\\
2 & -1 & 15 & -5\\
4 & 2 & 1 &  1\\
3 & 0 & 1 &  -4
\end{vmatrix}
}{-65}=\frac{-195}{-65}=3
$$

$$
w=\frac{\Delta_4}{\Delta}=
\frac{
\begin{vmatrix}
3 & 2 & 1& 4 \\
2 & -1 & 2 & 15\\
4 & 2 & 0 & 1 \\
3 & 0 &  -2 & 1
\end{vmatrix}
}{-65}=\frac{65}{-65}=-1
$$
%%%%%
%%%%%
\end{document}
